# baseURI: http://topbraid.org/sxml
# imports: http://www.topbraid.org/2007/05/composite.owl

# c14n-version: 3
@prefix owl: <http://www.w3.org/2002/07/owl#> .
@prefix rdf: <http://www.w3.org/1999/02/22-rdf-syntax-ns#> .
@prefix rdfs: <http://www.w3.org/2000/01/rdf-schema#> .
@prefix sxml: <http://topbraid.org/sxml#> .
@prefix xsd: <http://www.w3.org/2001/XMLSchema#> .
<http://topbraid.org/sxml>
  rdf:type owl:Ontology ;
  rdfs:comment """An ontology describing XML documents (elements and their hierarchy).
XML Documents have a root element. Attributes are represented as values of datatype properties that have a value for sxml:attribute. Future versions may also support object properties to resolve IDREF attributes. Elements are represented as instances of classes that have an sxml:element annotation.""" ;
  owl:imports <http://www.topbraid.org/2007/05/composite.owl> ;
  owl:versionInfo "1.2.0"^^xsd:string ;
.
sxml:CDATA
  rdf:type owl:Class ;
  rdfs:label "CDATA"^^xsd:string ;
  rdfs:subClassOf sxml:Node ;
.
sxml:Comment
  rdf:type owl:Class ;
  rdfs:label "Comment" ;
  rdfs:subClassOf sxml:Node ;
.
sxml:Document
  rdf:type owl:Class ;
  rdfs:label "Document" ;
  rdfs:subClassOf sxml:Node ;
.
sxml:Element
  rdf:type owl:Class ;
  rdfs:label "Element" ;
  rdfs:subClassOf sxml:Node ;
.
sxml:Node
  rdf:type owl:Class ;
  rdfs:label "Node" ;
  rdfs:subClassOf owl:Thing ;
.
sxml:TextNode
  rdf:type owl:Class ;
  rdfs:label "Text Node" ;
  rdfs:subClassOf sxml:Node ;
.
sxml:XSDValidationError
  rdf:type rdfs:Class ;
  rdfs:comment "Can be used to represent XML Schema validation errors. The rdfs:label contains details."^^xsd:string ;
  rdfs:label "XSD validation error"^^xsd:string ;
  rdfs:subClassOf rdfs:Resource ;
.
sxml:XSDValidationWarning
  rdf:type rdfs:Class ;
  rdfs:comment "Can be used to represent XML Schema validation warnings. The rdfs:label contains details."^^xsd:string ;
  rdfs:label "XSD validation warning"^^xsd:string ;
  rdfs:subClassOf rdfs:Resource ;
.
sxml:attribute
  rdf:type owl:AnnotationProperty ;
  rdfs:comment "The XML tag used to render an RDF property into an XML attribute. This must be a valid XML attribute name." ;
  rdfs:domain rdf:Property ;
  rdfs:label "attribute"^^xsd:string ;
.
sxml:element
  rdf:type owl:AnnotationProperty ;
  rdfs:comment "The XML tag used to render an element. The values of this property must be valid XML tag strings or URI resources that can be abbreviated by an existing namespace prefix. For example, a tag <process> would be mapped into a class with sxml:element=\"process\"^^xsd:string. A tag <my:process> would be mapped into a class with sxml:element=my:process (which is often identical to the URI of the class itself)." ;
  rdfs:domain rdfs:Class ;
  rdfs:label "element"^^xsd:string ;
.
sxml:isAttribute
  rdf:type owl:AnnotationProperty ;
  rdfs:comment "The XML tag used to mark if an OWL restriction should be generated as an XML attribute or simple content." ;
  rdfs:domain owl:Restriction ;
  rdfs:label "is attribute"^^xsd:string ;
  rdfs:range xsd:boolean ;
.
sxml:order
  rdf:type owl:AnnotationProperty ;
  rdfs:comment "The XML tag used for ordering. This is an annotation property that can be used to annotate both instance and non-instance resources." ;
  rdfs:domain rdfs:Resource ;
  rdfs:label "order"^^xsd:string ;
  rdfs:range xsd:int ;
.
sxml:prefix
  rdf:type owl:DatatypeProperty ;
  rdfs:comment "Stores the name of the prefixes that will be written back to the XML file when saved. This is mainly for round-tripping XML files that have xmlns... attributes in the root element." ;
  rdfs:label "prefix"^^xsd:string ;
  rdfs:range xsd:string ;
.
sxml:root
  rdf:type owl:ObjectProperty ;
  rdfs:comment "The root element of an XML document." ;
  rdfs:domain sxml:Document ;
  rdfs:subPropertyOf <http://www.topbraid.org/2007/05/composite.owl#child> ;
.
sxml:tag
  rdf:type owl:AnnotationProperty ;
  rdfs:comment "The tag of an XML object." ;
.
sxml:text
  rdf:type owl:DatatypeProperty ;
  rdfs:comment "The body of an XML TextNode." ;
  rdfs:domain sxml:TextNode ;
  rdfs:label "text"^^xsd:string ;
  rdfs:range xsd:string ;
.
