# baseURI: http://uispin.org/uidb
# imports: http://uispin.org/ui
# prefix: uidb

@prefix owl: <http://www.w3.org/2002/07/owl#> .
@prefix rdf: <http://www.w3.org/1999/02/22-rdf-syntax-ns#> .
@prefix rdfs: <http://www.w3.org/2000/01/rdf-schema#> .
@prefix spin: <http://spinrdf.org/spin#> .
@prefix spl: <http://spinrdf.org/spl#> .
@prefix ui: <http://uispin.org/ui#> .
@prefix uidb: <http://uispin.org/uidb#> .
@prefix xsd: <http://www.w3.org/2001/XMLSchema#> .

<http://spinrdf.org/arg#password>
  rdf:type rdf:Property ;
  rdfs:subPropertyOf <http://spinrdf.org/sp#arg> ;
.
<http://spinrdf.org/arg#sql>
  rdf:type rdf:Property ;
  rdfs:subPropertyOf <http://spinrdf.org/sp#arg> ;
.
<http://spinrdf.org/arg#url>
  rdf:type rdf:Property ;
  rdfs:subPropertyOf <http://spinrdf.org/sp#arg> ;
.
<http://spinrdf.org/arg#userName>
  rdf:type rdf:Property ;
  rdfs:subPropertyOf <http://spinrdf.org/sp#arg> ;
.
<http://spinrdf.org/arg#varName>
  rdf:type rdf:Property ;
  rdfs:subPropertyOf <http://spinrdf.org/sp#arg> ;
.
<http://uispin.org/uidb>
  rdf:type owl:Ontology ;
  rdfs:comment "An extension of SWP defining control elements operating on relational databases using JDBC." ;
  owl:imports <http://uispin.org/ui> ;
.
uidb:select
  rdf:type ui:NodeClass ;
  spin:constraint [
      rdf:type spl:Argument ;
      spl:optional "true"^^xsd:boolean ;
      spl:predicate <http://spinrdf.org/arg#password> ;
      spl:valueType xsd:string ;
      rdfs:comment "The password if needed. Falls back to TopBraid's secure storage mechanism if left empty." ;
    ] ;
  spin:constraint [
      rdf:type spl:Argument ;
      spl:optional "true"^^xsd:boolean ;
      spl:predicate <http://spinrdf.org/arg#userName> ;
      spl:valueType xsd:string ;
      rdfs:comment "The database user name (if needed for the connection)." ;
    ] ;
  spin:constraint [
      rdf:type spl:Argument ;
      spl:optional "true"^^xsd:boolean ;
      spl:predicate <http://spinrdf.org/arg#varName> ;
      spl:valueType xsd:string ;
      rdfs:comment "The name of the variable holding the result set. Defaults to \"rs\"." ;
    ] ;
  spin:constraint [
      rdf:type spl:Argument ;
      spl:predicate <http://spinrdf.org/arg#sql> ;
      spl:valueType xsd:string ;
      rdfs:comment "The SQL query string." ;
    ] ;
  spin:constraint [
      rdf:type spl:Argument ;
      spl:predicate <http://spinrdf.org/arg#url> ;
      spl:valueType xsd:string ;
      rdfs:comment "The URL of the database." ;
    ] ;
  rdfs:comment "Performs a SELECT query against a given JDBC database and produces a (SPARQL) result set that can be queried and walked through, for example using ui:forEach. The child elements can access the result set using the provided variable name (which defaults to ?rs)." ;
  rdfs:label "select" ;
  rdfs:subClassOf ui:ControlElement ;
.
uidb:update
  rdf:type ui:NodeClass ;
  spin:constraint [
      rdf:type spl:Argument ;
      spl:optional "true"^^xsd:boolean ;
      spl:predicate <http://spinrdf.org/arg#password> ;
      spl:valueType xsd:string ;
      rdfs:comment "The password if needed. Falls back to TopBraid's secure storage mechanism if left empty." ;
    ] ;
  spin:constraint [
      rdf:type spl:Argument ;
      spl:optional "true"^^xsd:boolean ;
      spl:predicate <http://spinrdf.org/arg#userName> ;
      spl:valueType xsd:string ;
      rdfs:comment "The database user name (if needed for the connection)." ;
    ] ;
  spin:constraint [
      rdf:type spl:Argument ;
      spl:predicate <http://spinrdf.org/arg#sql> ;
      spl:valueType xsd:string ;
      rdfs:comment "The SQL update string." ;
    ] ;
  spin:constraint [
      rdf:type spl:Argument ;
      spl:predicate <http://spinrdf.org/arg#url> ;
      spl:valueType xsd:string ;
      rdfs:comment "The URL of the database." ;
    ] ;
  rdfs:comment "Performs an UPDATE against a given JDBC database." ;
  rdfs:label "update" ;
  rdfs:subClassOf ui:ControlElement ;
.
